vacid/sparse_array_proof.v
@@ -1,3 +1,130 @@
+Set Implicit Arguments.
+Require Import LibCore.
+Require Import CFPrim CFTactics. (* todo: group as CF *)
+Require Import sparse_array_ml.
+
+(* Require Import FuncTactics.*)
+
+Notation "'Hexists' x1 x2 x3 x4 , H" := 
+  (Hexists x1, Hexists x2, Hexists x3, Hexists x4, H)
+  (at level 39, x1 ident, x2 ident, x3 ident, x4 ident, H at level 50) : heap_scope.
+Notation "'Hexists' x1 x2 x3 x4 x5 , H" := 
+  (Hexists x1, Hexists x2, Hexists x3, Hexists x4, Hexists x5, H)
+  (at level 39, x1 ident, x2 ident, x3 ident, x4 ident, x5 ident, H at level 50) : heap_scope.
+
+
+Class BagIndex T A := { index : T -> A -> Prop }.
+
+Instance int_index : BagIndex int int.
+Proof. intros. constructor. exact (fun n i => 0 <= i < n). Defined.
+
+Lemma int_index_def : forall (n i : int),
+  index n i = (0 <= i < n).
+Proof. auto. Qed. 
+
+Instance array_index : forall A, BagIndex (array A) int.
+Proof. intros. constructor. exact (fun t i => index (length t) i). Defined.
+
+Lemma array_index_def : forall A (t:array A) i,
+  index t i = (0 <= i < length t).
+Proof. auto. Qed. 
+
+Opaque int_index array_index.
+
+Notation "m \( x )" := (LibBag.read m x)
+  (at level 29, format "m \( x )") : container_scope.
+Notation "m \( x := v )" := (update m x v)
+  (at level 29, format "m \( x := v )") : container_scope.
+
+
+Parameter ml_array_get_spec : forall `{Inhabited a},
+  Spec ml_array_get (l:loc) (i:int) |R>> 
+    forall (t:array a), index t i ->
+    keep R (l ~> Array Id t) (\= t\(i)).
+
+Parameter ml_array_set_spec : forall a,
+  Spec ml_array_set (l:loc) (i:int) (v:a) |R>> 
+    forall (t:array a), index t i -> 
+    R (l ~> Array Id t) (# l ~> Array Id (t\(i:=v))).
+      (* (# Hexists t', l ~> Array Id t' \* [t' = t\(i:=v)]).*)
+
+Hint Extern 1 (RegisterSpec ml_array_get) => Provide ml_array_get_spec.
+Hint Extern 1 (RegisterSpec ml_array_set) => Provide ml_array_set_spec.
+
+
+Ltac xchange_debug L :=
+  let K := fresh "TEMP" in
+  forwards_nounfold K: L; eapply xchange_lemma; 
+    [ clear K; try xlocal
+    | apply K
+    | clear K; instantiate 
+    | clear K ].
+
+
+(****************************************************)
+(* Specification of the invariant *)
+
+Definition tab := array int.
+
+Definition L := maxlen.
+
+Definition SarrayPacked :=
+  @Sarray int (array int) (array int) (array int) Id (Array Id) (Array Id) (Array Id).
+Definition SarrayUnpacked :=
+  @Sarray int loc loc loc Id Id Id Id.
+
+Definition SparseArray (T:tab) (s:loc) :=
+  Hexists (n:int) (Val:tab) (Idx:tab) (Back:tab),
+     s ~> SarrayPacked n Val Idx Back
+  \* [ length Val = L /\ length Idx = L /\ length Back = L 
+       /\ forall k, index n k -> let i := Back\(k) in
+          index L i  /\  Idx\(i) = k  /\  T\(k) = Val\(k) ].
+
+
+Lemma valid_spec :
+  Spec valid i s |R>> forall n Val Idx Back,
+    keep R (s ~> SarrayPacked n Val Idx Back)
+           (\[ bool_of (index L i /\ Back\(Idx\(i)) = i) ]).
+Proof.
+  xcf. intros.
+  unfold SarrayPacked.
+  xchange (Sarray_focus s). xextract as n' val idx back.
+(*  xpost.*)
+  xif.
+  (* case in bound *)
+  xapps.
+  xapps.
+  (* case not in bound *)
+  xchange (Sarray_unfocus s n' val idx back).
+  xret. hsimpl. xclean. rew_reflect in *.
+    intros [H _]. apply C. rewrite int_index_def in H. 
+    split; fold_prop; unfolds L; try math.
+
+ (*--todo :sortir le n' ~> Id n *)
+Qed.
+
+let valid i s =
+   0 <= i && i < maxlen && s.back.(s.idx.(i)) = i
+
+
+Lemma get_spec :
+  Spec get i s |R>> forall T, index T i -> 
+    keep R (s ~> SparseArray T) (\= T\(i)).
+Proof.
+  xcf. introv Ii.
+  xlet. 
+
+Qed.
+
+    
+
+
+
+
+
+
+---------
+
 Definition L := maxlen.
 
 Definition idx_back_coherent n Back Idx :=
